Models/Finite/RelyGuarantee3.thy
@@ -1,0 +1,97 @@
+theory RelyGuarantee3
+  imports Language
+begin
+
+datatype 'a act = Act "'a set" "'a rel"
+
+fun eval_word :: "'a act list \<Rightarrow> 'a set \<Rightarrow> 'a set" where
+  "eval_word [] p = p"
+| "eval_word (Act q x # xs) p = (if p \<subseteq> q then eval_word xs (x `` p) else {})"
+
+lemma eval_word_empty [simp]: "eval_word xs {} = {}"
+proof (induct xs)
+  case Nil show ?case by simp
+next
+  case (Cons x xs) thus ?case by (cases x) simp
+qed
+
+lemma eval_append_word: "eval_word (xs @ ys) h = eval_word ys (eval_word xs h)"
+proof (induct xs arbitrary: h)
+  case Nil show ?case by simp
+next
+  case (Cons x xs) thus ?case
+    by (cases x) simp
+qed
+
+lemma Image_continuous: "x `` (\<Union>X) = \<Union>Image x ` X"
+  by auto
+
+lemma eval_word_continuous: "eval_word w (\<Union>X) \<subseteq> \<Union>(eval_word w ` X)"
+proof (induct w arbitrary: X)
+  case Nil show ?case by simp
+next
+  case (Cons x xs)
+  show ?case
+  proof (induct x)
+    fix p x
+    {
+      assume "\<Union>X \<subseteq> p"
+      hence "eval_word (Act p x # xs) (\<Union>X) \<subseteq> \<Union> (eval_word (Act p x # xs) ` X)"
+        apply (simp add: image_def)
+        apply (subst Image_continuous)
+        apply (rule order_trans[OF Cons.hyps])
+        by auto
+    }
+    moreover
+    {
+      assume "\<not> (\<Union>X \<subseteq> p)"
+      hence "eval_word (Act p x # xs) (\<Union>X) \<subseteq> Sup (eval_word (Act p x # xs) ` X)"
+        by simp
+    }
+    ultimately show "eval_word (Act p x # xs) (\<Union>X) \<subseteq> Sup (eval_word (Act p x # xs) ` X)"
+      by blast
+  qed
+qed
+
+definition module :: "'a act lan \<Rightarrow> 'a set \<Rightarrow> 'a set" (infix "\<Colon>" 60) where
+  "x \<Colon> h = Sup {eval_word w h|w. w \<in> x}"
+
+lemma (in complete_lattice) Sup_comp_mono [intro]: "(\<And>x. P x \<Longrightarrow> f x \<le> g x) \<Longrightarrow> Sup {f x |x. P x} \<le> Sup {g x |x. P x}"
+  by (auto intro: Sup_mono)
+
+lemma (in complete_lattice) Sup_comp_conj: "Sup {f x y |x y. P x \<and> Q y} = Sup {Sup {f x y |x. P x} |y. Q y}"
+  apply (rule antisym)
+  apply (simp_all add: Sup_le_iff)
+  apply auto
+  defer
+  apply (rule Sup_mono)
+  apply auto
+  apply (subgoal_tac "f x y \<le> Sup {f x y |y. Q y}")
+  apply (erule order_trans)
+  defer
+  apply (metis (lifting, full_types) Sup_upper mem_Collect_eq)
+  apply (rule Sup_comp_mono)
+  by (metis (lifting, full_types) Sup_upper mem_Collect_eq)
+
+lemma mod_mult: "y \<Colon> (x \<Colon> h) \<subseteq> x\<cdot>y \<Colon> h"
+proof -
+  have "y \<Colon> (x \<Colon> h) = \<Union>{eval_word yw (x \<Colon> h)|yw. yw \<in> y}"
+    by (simp add: module_def)
+  also have "... = \<Union>{eval_word yw (\<Union>{eval_word xw h|xw. xw \<in> x})|yw. yw \<in> y}"
+    by (simp add: module_def)
+  also have "... \<subseteq> \<Union>{\<Union>{eval_word yw (eval_word xw h)|xw. xw \<in> x}|yw. yw \<in> y}"
+    apply (rule Sup_comp_mono)
+    apply (rule order_trans[OF eval_word_continuous])
+    by (auto simp add: image_def)
+  also have "... = \<Union>{eval_word yw (eval_word xw h)|xw yw. xw \<in> x \<and> yw \<in> y}"
+    by blast
+  also have "... = \<Union>{eval_word (xw @ yw) h|xw yw. xw \<in> x \<and> yw \<in> y}"
+    by (simp add: eval_append_word)
+  also have "... = \<Union>{eval_word w h|w. w \<in> x\<cdot>y}"
+    by (auto simp add: l_prod_def complex_product_def)
+  also have "... = x\<cdot>y \<Colon> h"
+    by (simp add: module_def)
+  finally show ?thesis .
+qed
+
+end
